Adressing the comments from the RP

code/sha3/Hacl.Impl.SHA3.fst
@@ -378,21 +378,21 @@ let storeState rateInBytes s res =
     )
 
 (* 
-   Lemma_equivalence_state_rate proves that it is equivalent
+   Lemma lemma_equiv_alloc_bigger_state proves that it is equivalent
    to allocate a bigger temporary buffer and then use a part of it 
    compared to allocation of the exact size buffer *)
 
-val lemma_equiv_alloc_bigger_state: #l: size_nat -> a:size_t{v a > 0 /\ v a <= l} 
+val lemma_equiv_alloc_bigger_state: #len: size_nat -> #t: inttype -> #l: secrecy_level 
+  -> a:size_t{v a > 0 /\ v a <= len} 
   -> Lemma (
-    let input0 = Lib.Sequence.create #uint8 (v a) (u8 0) in
-    let nextBlock_1 = Lib.Sequence.create #uint8 l (u8 0) in 
-    let input1 = Lib.Sequence.sub #uint8 #l nextBlock_1 0 (v a) in 
+    let input0 = Lib.Sequence.create #(int_t t l) (v a) (mk_int #t #l 0) in
+    let nextBlock_1 = Lib.Sequence.create #(int_t t l) len (mk_int #t #l 0) in 
+    let input1 = Lib.Sequence.sub #(int_t t l) #len nextBlock_1 0 (v a) in 
     input0 == input1)
-
-let lemma_equiv_alloc_bigger_state #l a  = 
-  let input0 = Lib.Sequence.create #uint8 (v a) (u8 0) in
-  let nextBlock_1 = Lib.Sequence.create #uint8 l (u8 0) in 
-  let input1 = Lib.Sequence.sub #uint8 #l nextBlock_1 0 (v a) in 
+let lemma_equiv_alloc_bigger_state #len #t #l a  = 
+  let input0 = Lib.Sequence.create #(int_t t l) (v a) (mk_int #t #l 0) in
+  let nextBlock_1 = Lib.Sequence.create #(int_t t l) len (mk_int #t #l 0) in 
+  let input1 = Lib.Sequence.sub #(int_t t l) #len nextBlock_1 0 (v a) in 
   Seq.lemma_eq_intro input0 input1
 
 
@@ -416,8 +416,7 @@ let absorb_next s rateInBytes =
       nextBlock.(rateInBytes -! 1ul) <- u8 0x80;
       loadState rateInBytes nextBlock s;
       state_permute s;
-      lemma_equiv_alloc_bigger_state #200 rateInBytes)
-
+      lemma_equiv_alloc_bigger_state #200 #U8 #SEC rateInBytes)
 
 inline_for_extraction noextract
 val absorb_last_:
@@ -450,16 +449,16 @@ let absorb_last_ delimitedSuffix rateInBytes rem input s =
          (size_to_UInt32 rem = size_to_UInt32 (rateInBytes -. 1ul))
       then state_permute s;
       absorb_next s rateInBytes;
-      lemma_equiv_alloc_bigger_state #200 rateInBytes)
+      lemma_equiv_alloc_bigger_state #200 #U8 #SEC rateInBytes)
 
-val compare_more_zero_lte_b: a: size_t -> b: size_t -> Tot (r: bool {
+private
+inline_for_extraction noextract
+val positive_and_lte: a: size_t -> b: size_t -> Tot (r: bool {
   r == not (v a > 0 && v a <= v b)})
-
-let compare_more_zero_lte_b a b = 
+let positive_and_lte a b = 
   let a_is_zero = eq a (size 0) in 
   let a_lte_200 = gt a b in 
   a_is_zero || a_lte_200
-
 
 val absorb_last:
     delimitedSuffix:byte_t
@@ -469,24 +468,22 @@ val absorb_last:
   -> s:state
   -> Stack bool
     (requires fun h -> live h s /\ live h input /\ disjoint s input)
-    (ensures  fun h0 flag h1 ->
+    (ensures  fun h0 success h1 ->
       modifies (loc s) h0 h1 /\ (
       if v rateInBytes > 0 && v rateInBytes <= 200 && v rem < v rateInBytes then
-	flag /\
+	success /\
 	as_seq h1 s ==
 	S.absorb_last delimitedSuffix (v rateInBytes) (v rem)
           (as_seq h0 input) (as_seq h0 s)
       else 
-	~flag))
-		
+	~ success))
 let absorb_last delimitedSuffix rateInBytes rem input s =
-  if compare_more_zero_lte_b rateInBytes (size 200) || gte rem rateInBytes then 
+  if positive_and_lte rateInBytes (size 200) || gte rem rateInBytes then 
     false
   else begin
     absorb_last_ delimitedSuffix rateInBytes rem input s; 
     true
   end
-  
 
 inline_for_extraction noextract
 val absorb_inner_:
@@ -503,30 +500,27 @@ let absorb_inner_ rateInBytes block s =
   loadState rateInBytes block s;
   state_permute s
 
-
 val absorb_inner:
     rateInBytes:size_t
   -> block:lbuffer uint8 rateInBytes
   -> s:state
   -> Stack bool
     (requires fun h0 -> live h0 s /\ live h0 block /\ disjoint s block)
-    (ensures  fun h0 flag h1 ->
+    (ensures  fun h0 success h1 ->
       modifies (loc s) h0 h1 /\ (
       if v rateInBytes > 0 && v rateInBytes <= 200 then
-	flag /\
+	success /\
 	as_seq h1 s ==
 	S.absorb_inner (v rateInBytes) (as_seq h0 block) (as_seq h0 s)
       else
-	~ flag))
-	
+	~ success))
 let absorb_inner rateInBytes block s =
-  if compare_more_zero_lte_b rateInBytes (size 200) then 
+  if positive_and_lte rateInBytes (size 200) then 
     false
   else begin
     absorb_inner_ rateInBytes block s;
     true
   end
-
 
 inline_for_extraction noextract
 val absorb_:
@@ -542,14 +536,12 @@ val absorb_:
       as_seq h1 s ==
       S.absorb (as_seq h0 s) (v rateInBytes) (v inputByteLen)
         (as_seq h0 input) delimitedSuffix)
-	
 let absorb_ s rateInBytes inputByteLen input delimitedSuffix =
   loop_blocks rateInBytes inputByteLen input
   (S.absorb_inner (v rateInBytes))
   (S.absorb_last delimitedSuffix (v rateInBytes))
   (absorb_inner_ rateInBytes)
   (absorb_last_ delimitedSuffix rateInBytes) s
-
 
 val absorb:
     s:state
@@ -559,18 +551,18 @@ val absorb:
   -> delimitedSuffix:byte_t
   -> Stack bool
     (requires fun h0 -> live h0 s /\ live h0 input /\ disjoint s input)
-    (ensures  fun h0 flag h1 ->
+    (ensures fun h0 success h1 ->
       modifies (loc s) h0 h1 /\ (
       if v rateInBytes > 0 && v rateInBytes <= 200 then 
-	flag /\
+	success /\
 	as_seq h1 s ==
 	S.absorb (as_seq h0 s) (v rateInBytes) (v inputByteLen)
           (as_seq h0 input) delimitedSuffix
       else
-	~flag ))
+	~ success ))
 
 let absorb s rateInBytes inputByteLen input delimitedSuffix = 
-  if compare_more_zero_lte_b rateInBytes (size 200) then 
+  if positive_and_lte rateInBytes (size 200) then 
     false
   else begin
     absorb_ s rateInBytes inputByteLen input delimitedSuffix;
@@ -639,27 +631,24 @@ val squeeze:
   -> output:lbuffer uint8 outputByteLen
   -> Stack bool
     (requires fun h0 -> live h0 s /\ live h0 output /\ disjoint s output)
-    (ensures  fun h0 flag h1 ->
+    (ensures  fun h0 success h1 ->
       modifies2 s output h0 h1 /\ (
       if v rateInBytes > 0 && v rateInBytes <= 200 then 
-	flag /\
+	success /\
 	as_seq h1 output == S.squeeze (as_seq h0 s) (v rateInBytes) (v outputByteLen)
       else
-	~flag ))
-
+	~success ))
 let squeeze s rateInBytes outputByteLen output = 
-  if compare_more_zero_lte_b rateInBytes (size 200) then 
+  if positive_and_lte rateInBytes (size 200) then 
     false
   else begin
     squeeze_ s rateInBytes outputByteLen output;
     true
   end
 
-
 inline_for_extraction noextract
 val keccak_:
     rate:size_t{v rate % 8 == 0 /\ v rate / 8 > 0 /\ v rate <= 1600}
-  -> capacity:size_t{v capacity + v rate == 1600}
   -> inputByteLen:size_t
   -> input:lbuffer uint8 inputByteLen
   -> delimitedSuffix:byte_t
@@ -668,10 +657,11 @@ val keccak_:
   -> Stack unit
     (requires fun h -> live h input /\ live h output /\ disjoint input output)
     (ensures  fun h0 _ h1 ->
-      modifies1 output h0 h1 /\
+      modifies1 output h0 h1 /\ (
+      let capacity = 1600 - v rate in 
       as_seq h1 output ==
-      S.keccak (v rate) (v capacity) (v inputByteLen) (as_seq h0 input) delimitedSuffix (v outputByteLen))
-let keccak_ rate capacity inputByteLen input delimitedSuffix outputByteLen output =
+      S.keccak (v rate) capacity (v inputByteLen) (as_seq h0 input) delimitedSuffix (v outputByteLen)))
+let keccak_ rate inputByteLen input delimitedSuffix outputByteLen output =
   push_frame();
   let rateInBytes = rate /. size 8 in
   let s:state = create 25ul (u64 0) in
@@ -679,10 +669,8 @@ let keccak_ rate capacity inputByteLen input delimitedSuffix outputByteLen outpu
   squeeze_ s rateInBytes outputByteLen output;
   pop_frame()
 
-
 val keccak:
     rate:size_t
-  -> capacity:size_t
   -> inputByteLen:size_t
   -> input:lbuffer uint8 inputByteLen
   -> delimitedSuffix:byte_t
@@ -690,39 +678,26 @@ val keccak:
   -> output:lbuffer uint8 outputByteLen
   -> Stack bool
     (requires fun h -> live h input /\ live h output /\ disjoint input output)
-    (ensures  fun h0 flag h1 ->
+    (ensures  fun h0 success h1 ->
       modifies1 output h0 h1 /\ (
-      if v rate % 8 = 0 && v rate / 8 > 0 && v rate <= 1600 && v capacity + v rate = 1600 then
-	flag /\ 
+      let capacity = 1600 - v rate in 
+      if v rate % 8 = 0 && v rate / 8 > 0 && v rate <= 1600 then
+	success /\ 
 	as_seq h1 output ==
-	S.keccak (v rate) (v capacity) (v inputByteLen) (as_seq h0 input) delimitedSuffix (v outputByteLen)
+	S.keccak (v rate) capacity (v inputByteLen) (as_seq h0 input) delimitedSuffix (v outputByteLen)
       else
-	~ flag))
-
-let keccak rate capacity inputByteLen input delimitedSuffix outputByteLen output = 
+	~ success))
+let keccak rate inputByteLen input delimitedSuffix outputByteLen output = 
   let bit3mask = size 7 in 
   let rate_mod_8 = eq (logand rate bit3mask) (size 0) in 
-    logand_mask rate bit3mask 3;
-    
+    logand_mask rate bit3mask 3;  
   let rateInBytes = rate /. size 8 in 
   let rate_is_zero = eq rateInBytes (size 0) in 
   let rate_lte_200 = gt rateInBytes (size 200) in 
-  
   if not rate_mod_8 || (rate_is_zero) || rate_lte_200 then begin
     false 
     end
   else begin
-    assert(v rate % 8 = 0 && v rate / 8 > 0 && v rate <= 1600);
-    let capacity_less_flag = gt capacity (size 1600) in 
-    if capacity_less_flag then 
-      false 
-    else begin
-      let capacity_and_rate_equal_1600 = eq (add capacity rate) (size 1600) in 
-      if not capacity_and_rate_equal_1600 then 
-	 false
-      else begin
-	keccak_ rate capacity inputByteLen input delimitedSuffix outputByteLen output;
-	true
-    end
-    end
+    keccak_ rate inputByteLen input delimitedSuffix outputByteLen output;
+    true
   end
